automatic.v
@@ -1,0 +1,100 @@
+(* Decision procedures for linear integer arithmetic. *)
+
+Require Vector.
+Require Import Utf8 Nat BinNat List.
+From larith Require Import tactics notations utilities.
+From larith Require Import formulae automata.
+Import ListNotations.
+
+(* Definition of a regular predicate. *)
+Section Regular_predicates.
+
+Record regular (letter : Set) (P : list letter -> Prop) := Regular {
+  r_automaton : automaton letter;
+  r_size      : nat;
+  r_finite    : Finite r_automaton r_size;
+  r_dec       : ∀s t : state r_automaton, {s = t} + {s ≠ t};
+  r_spec      : ∀w, Language r_automaton w <-> P w;
+}.
+
+(* Regular predicates can be decided. *)
+Theorem regular_dec letter P :
+  regular letter P -> {∃w, P w} + {∀w, ¬P w}.
+Proof.
+Admitted.
+
+End Regular_predicates.
+
+(* Finite-length vectors form a finite alphabet. *)
+Section Finite_vector_alphabet.
+
+Fixpoint enumerate_vectors n : list (vec n) :=
+  match n with
+  | 0 => [⟨⟩]
+  | S m =>
+    let vs := enumerate_vectors m in
+    map (vcons false m) vs ++
+    map (vcons true m) vs
+  end.
+
+Theorem enumerate_vectors_spec n (v : vec n) :
+  In v (enumerate_vectors n).
+Proof.
+induction v; simpl. now left.
+apply in_app_iff; destruct h; [right|left]; apply in_map, IHv.
+Qed.
+
+End Finite_vector_alphabet.
+
+(* Transpose a vector list. *)
+Section Matrix_transposition.
+
+Variable T : Type.
+
+(* Convert from a list of collumn vectors to a vector of row lists. *)
+Fixpoint transpose {n} (w : list (Vector.t T n)) : Vector.t (list T) n :=
+  match w with
+  | [] => Vector.const [] n
+  | v :: w' => Vector.map2 cons v (transpose w')
+  end.
+
+Theorem transpose_cons {n} (w : list (Vector.t T (S n))) :
+  transpose w = map Vector.hd w ;; transpose (map Vector.tl w).
+Proof.
+induction w; simpl. easy.
+apply Vector.caseS' with (v:=a).
+intros; now rewrite IHw.
+Qed.
+
+End Matrix_transposition.
+
+Arguments transpose {_ _}.
+
+(* Algorithm for deciding first-order realizability using finite automata. *)
+Section Decide_wff_using_automata.
+
+Variable atom domain : Type. 
+Variable value : list bool -> domain.
+Variable Model : model atom domain.
+
+Definition vctx {n} (w : list (vec n)) : list domain :=
+  map value (Vector.to_list (transpose w)).
+
+Hypothesis hypothesis :
+  ∀a, Σ n, regular (vec n) (λ w, Model (vctx w) a).
+
+Theorem wff_regular φ :
+  Σ n, regular (vec n) (λ w, Model |= (φ)[vctx w]).
+Proof.
+induction φ; simpl.
+- (* Atomic formulae: we assume these are regular. *)
+  apply hypothesis.
+- (* Conjunction: project on a common alphabet, and use the product. *)
+  admit.
+- (* Negation: apply determinization and use the complement. *)
+  admit.
+- (* Quantification: use tail projection, and find a witness in the image. *)
+  admit.
+Abort.
+
+End Decide_wff_using_automata.
