notations.v
@@ -1,6 +1,6 @@
 (* General purpose notations. *)
 
-Require Import Utf8.
+Require Import Utf8 Vector.
 
 (* Sigma types. *)
 Notation "'Σ' x .. y , P" := (sigT (λ x, .. (sigT (λ y, P)) ..))
@@ -9,3 +9,16 @@ Notation "'Σ' x .. y , P" := (sigT (λ x, .. (sigT (λ y, P)) ..))
 
 (* Cartesian products. *)
 Notation "A × B" := (prod A B) (at level 100).
+
+(* Vectors. *)
+Notation vec := (Vector.t bool).
+Notation vnil := (Vector.nil _).
+Notation vcons := (Vector.cons _).
+
+Notation "⟨ ⟩" := (vnil) (format "⟨ ⟩").
+Notation "h ;; t" := (vcons h _ t)
+  (at level 60, right associativity, format "h  ;;  t").
+
+Notation "⟨ x ⟩" := (x ;; ⟨⟩).
+Notation "⟨ x ; y ; .. ; z ⟩" :=
+  (vcons x _ (vcons y _ .. (vcons z _ (nil _)) ..)).
